add a low* implementation of SHA3 and test

specs/Spec.Keccak.fst
@@ -6,90 +6,116 @@ open Lib.Sequence
 open Lib.ByteSequence
 open FStar.Mul
 
-let lfsr86540 (lfsr:uint8) : tuple2 uint8 bool =
-  let lfsr1 : uint8 = logand #U8 lfsr (u8 1) in
-  let result : bool = u8_to_UInt8 lfsr1 <> 0uy in
-  let lfsr' : uint_t U8 = shift_left #U8 lfsr (u32 1) in
-  if (u8_to_UInt8 (logand #U8 lfsr (u8 0x80)) <> 0uy) then
-    (logxor #U8 lfsr' (u8 0x71)), result
-  else
-    lfsr', result
-
 type state = lseq uint64 25
 type index = n:size_nat{n < 5}
 
-let readLane (s:state) (x:index) (y:index) : uint64 = 
+let lfsr86540 (lfsr:uint8) : tuple2 uint8 bool =
+  let lfsr1 = lfsr &. u8 1 in
+  let result = u8_to_UInt8 lfsr1 <> 0uy in
+  let lfsr' = lfsr <<. u32 1 in
+  if u8_to_UInt8 (lfsr &. u8 0x80) <> 0uy then
+    lfsr' ^. u8 0x71, result
+  else
+    lfsr', result
+
+let readLane (s:state) (x:index) (y:index) : uint64 =
   s.[x + 5 * y]
 
-let writeLane (s:state ) (x:index) (y:index) (v:uint64) : state = 
+let writeLane (s:state ) (x:index) (y:index) (v:uint64) : state =
   s.[x + 5 * y] <- v
 
-#set-options "--max_fuel 0 --z3rlimit 100"
+#set-options "--z3rlimit 100 --max_fuel 0 --max_ifuel 0"
 
-let state_permute1 (s:state) (lfsr:uint8) : tuple2 state uint8 =
+let state_theta (s:state) : state  =
   let _C = create 5 (u64 0) in
   let _C =
     repeati 5 (fun x _C ->
-      _C.[x] <- readLane s x 0 ^. readLane s x 1 ^. readLane s x 2 ^. readLane s x 3 ^. readLane s x 4) _C in
-  let s_theta =
-    repeati 5 (fun x s ->
-      let _D = _C.[(x+4)%5] ^. (_C.[(x+1)%5] <<<. (u32 1)) in
-      repeati 5 (fun y s ->
-        writeLane s x y (logxor #U64 (readLane s x y) _D)) s) s in
+      _C.[x] <-
+	readLane s x 0 ^.
+	readLane s x 1 ^.
+	readLane s x 2 ^.
+	readLane s x 3 ^.
+	readLane s x 4
+    ) _C in
+  repeati 5 (fun x s ->
+    let _D = _C.[(x + 4) % 5] ^. (_C.[(x + 1) % 5] <<<. u32 1) in
+    repeati 5 (fun y s ->
+      writeLane s x y (readLane s x y ^. _D)
+    ) s
+  ) s
 
+let state_pi_rho (s_theta:state) : state  =
   let x : index = 1 in
   let y : index = 0 in
   let current : uint64 = readLane s_theta x y in
-  let (_,_,_,s_pi_rho) =
+  let _, _, _, s_pi_rho =
     repeati 24 (fun t (tup: tuple4 index index uint64 state) ->
-      let (x,y,current,s) = tup in
-      let r : uint32 = u32 (((t + 1) * (t + 2)/2) % 64) in
-      let _Y: index = ((2 * x + 3 * y) % 5) in
+      let x, y, current, s = tup in
+      let r : r:uint32{uint_v r < 64} = u32 (((t + 1) * (t + 2) / 2) % 64) in
+      let _Y: index = (2 * x + 3 * y) % 5 in
       let x = y in
       let y = _Y in
       let temp = readLane s x y in
-      let s = writeLane s x y (rotate_left #U64 current r) in
+      let s = writeLane s x y (current <<<. r) in
       let current = temp in
-      (x,y,current,s)) (x,y,current,s_theta) in
+      x, y, current, s
+    ) (x, y, current, s_theta) in
+  s_pi_rho
 
+let state_chi (s_pi_rho:state) : state  =
   let temp = s_pi_rho in
-  let s_chi =
-    repeati 5 (fun y s ->
-      repeati 5 (fun x s ->
-        writeLane s x y ((readLane temp x y) ^. (logand #U64 (lognot (readLane temp ((x+1)%5) y)) (readLane temp ((x+2)%5) y)))) s) s_pi_rho in
-							
-  let (s_iota,lfsr) =
-    repeati 7 (fun j (s,lfsr) ->
-      Math.Lemmas.pow2_le_compat 6 j;
-      assert_norm (pow2 6 = 64);
-      let bitPosition = u32 ((pow2 j) - 1) in
-      let (lfsr,result) = lfsr86540 lfsr in
-      if result then
-        (writeLane s 0 0 (logxor #U64 (readLane s 0 0) (shift_left #U64 (u64 1) bitPosition)), lfsr)
-      else (s,lfsr)) (s_chi,lfsr) in
-  (s_iota,lfsr)
+  repeati 5 (fun y s ->
+    repeati 5 (fun x s ->
+      writeLane s x y
+	(readLane temp x y ^.
+	((lognot (readLane temp ((x + 1) % 5) y)) &. readLane temp ((x + 2) % 5) y))
+    ) s
+  ) s_pi_rho
+
+let state_iota (s_chi:state) (lfsr:uint8) : tuple2 state uint8 =
+  repeati 7 (fun j (s, lfsr) ->
+    Math.Lemmas.pow2_le_compat 6 j;
+    assert_norm (pow2 6 = 64);
+    let bitPosition = u32 (pow2 j - 1) in
+    let lfsr, result = lfsr86540 lfsr in
+    if result then
+      writeLane s 0 0 (readLane s 0 0 ^. (u64 1 <<. bitPosition)), lfsr
+    else s, lfsr
+  ) (s_chi, lfsr)
+
+let state_permute1 (s:state) (lfsr:uint8) : tuple2 state uint8 =
+  let s_theta = state_theta s in
+  let s_pi_rho = state_pi_rho s_theta in
+  let s_chi = state_chi s_pi_rho in
+  let s_iota, lfsr = state_iota s_chi lfsr in
+  s_iota, lfsr
 
 let state_permute (s:state) : state =
   let lfsr = u8 0x01 in
-  let (s,lfsr) = repeat 24 (fun (s,lfsr) -> state_permute1 s lfsr) (s,lfsr) in
+  let s, lfsr =
+    repeat 24 (fun (s, lfsr) ->
+      state_permute1 s lfsr
+    ) (s, lfsr) in
   s
 
 let loadState (rateInBytes:size_nat{rateInBytes <= 200})
 	      (input:lbytes rateInBytes)
 	      (s:state) : state =
   let block = create 200 (u8 0) in
-  let block = update_slice block 0 rateInBytes input in
+  let block = update_sub block 0 rateInBytes input in
   repeati 25 (fun j s ->
-    let nj = uint_from_bytes_le #U64 (slice block (j*8) ((j*8) + 8)) in
-    s.[j] <- (s.[j] ^. nj) ) s
+    let nj = uint_from_bytes_le #U64 (sub block (j * 8) 8) in
+    s.[j] <- s.[j] ^. nj
+  ) s
 
 let storeState (rateInBytes:size_nat{rateInBytes <= 200})
 	       (s:state) : lbytes rateInBytes =
   let block = create 200 (u8 0) in
   let block =
     repeati 25 (fun j block ->
-      update_slice block (j * 8) (j*8 + 8) (uint_to_bytes_le #U64 s.[j])) block in
-  slice block 0 rateInBytes
+      update_sub block (j * 8) 8 (uint_to_bytes_le #U64 s.[j])
+    ) block in
+  sub block 0 rateInBytes
 
 let absorb (s:state)
            (rateInBytes:size_nat{rateInBytes > 0 /\ rateInBytes <= 200})
@@ -99,18 +125,19 @@ let absorb (s:state)
   let n = inputByteLen / rateInBytes in
   let s : state =
     repeati n (fun i s ->
-	  let s = loadState rateInBytes (slice input (i*rateInBytes) (i*rateInBytes + rateInBytes)) s in
-	  state_permute s) s in
+      let s = loadState rateInBytes (sub input (i * rateInBytes) rateInBytes) s in
+      state_permute s
+    ) s in
   let rem = inputByteLen % rateInBytes in
-  let last: lseq uint8 rem = slice input (inputByteLen - rem) inputByteLen in
+  let last: lseq uint8 rem = sub input (inputByteLen - rem) rem in
   let lastBlock = create rateInBytes (u8 0) in
-  let lastBlock = update_slice lastBlock 0 rem last in
+  let lastBlock = update_sub lastBlock 0 rem last in
   let lastBlock = lastBlock.[rem] <- delimitedSuffix in
   let s = loadState rateInBytes lastBlock s in
 
-  let s = if (not (u8_to_UInt8 (logand #U8 delimitedSuffix (u8 0x80)) = 0uy) && (rem = rateInBytes - 1))
-	  then state_permute s
-	  else s in
+  let s =
+    if (not (u8_to_UInt8 (delimitedSuffix &. u8 0x80) = 0uy) && (rem = rateInBytes - 1))
+    then state_permute s else s in
   let nextBlock = create rateInBytes (u8 0) in
   let nextBlock = nextBlock.[rateInBytes - 1] <- u8 0x80 in
   let s = loadState rateInBytes nextBlock s in
@@ -119,19 +146,20 @@ let absorb (s:state)
 
 let squeeze (s:state)
 	    (rateInBytes:size_nat{rateInBytes > 0 /\ rateInBytes <= 200})
-	    (outputByteLen: size_nat)
+	    (outputByteLen:size_nat)
 	    : lbytes outputByteLen =
   let output = create outputByteLen (u8 0) in
   let outBlocks = outputByteLen / rateInBytes in
-  let (s, output) =
-    repeati outBlocks (fun i (s,o) ->
+  let s, output =
+    repeati outBlocks (fun i (s, o) ->
       let block = storeState rateInBytes s in
-      let o = update_slice o (i*rateInBytes) (i*rateInBytes + rateInBytes) block in
+      let o = update_sub o (i * rateInBytes) rateInBytes block in
       let s = state_permute s in
-      (s,o)) (s,output) in
+      s, o
+    ) (s, output) in
   let remOut = outputByteLen % rateInBytes in
   let outBlock = storeState remOut s in
-  update_slice output (outputByteLen - remOut) outputByteLen outBlock
+  update_sub output (outputByteLen - remOut) remOut outBlock
 
 let keccak (rate:size_nat{rate % 8 == 0 /\ rate / 8 > 0 /\ rate <= 1600})
 	   (capacity:size_nat{capacity + rate == 1600})
@@ -141,7 +169,7 @@ let keccak (rate:size_nat{rate % 8 == 0 /\ rate / 8 > 0 /\ rate <= 1600})
 	   (outputByteLen:size_nat)
 	   : lbytes outputByteLen =
   let rateInBytes : size_nat = rate / 8 in
-  let s : state = create 25 (u64 0) in  
+  let s : state = create 25 (u64 0) in
   let s = absorb s rateInBytes inputByteLen input delimitedSuffix in
   squeeze s rateInBytes outputByteLen
 
