code/experimental/sha3/Hacl.Impl.SHA3.fst
@@ -1,0 +1,351 @@
+module Hacl.Impl.SHA3
+
+open FStar.HyperStack.All
+open FStar.HyperStack
+open FStar.HyperStack.ST
+open FStar.Mul
+
+open LowStar.Buffer
+open LowStar.BufferOps
+
+open Lib.IntTypes
+open Lib.PQ.Buffer
+open Lib.Endianness
+
+module ST = FStar.HyperStack.ST
+module HS = FStar.HyperStack
+module B = LowStar.Buffer
+
+#reset-options "--z3rlimit 50 --max_fuel 0 --max_ifuel 0 --using_facts_from '* -FStar.Seq'"
+
+inline_for_extraction noextract
+let lbytes len = lbuffer uint8 len
+
+inline_for_extraction noextract
+let v = size_v
+
+inline_for_extraction noextract
+let state = lbuffer uint64 25
+
+inline_for_extraction noextract
+let index = n:size_t{v n < 5}
+
+let lfsr86540 (lfsr:uint8) : tuple2 uint8 bool =
+  let open Lib.RawIntTypes in
+  let lfsr1 = lfsr &. u8 1 in
+  let result = u8_to_UInt8 lfsr1 <> 0uy in
+  let lfsr' = lfsr <<. u32 1 in
+  if u8_to_UInt8 (lfsr &. u8 0x80) <> 0uy then
+    lfsr' ^. u8 0x71, result
+  else
+    lfsr', result
+
+inline_for_extraction noextract
+val readLane:
+     s:state
+  -> x:index
+  -> y:index
+  -> Stack uint64
+    (requires fun h -> live h s)
+    (ensures  fun h0 r h1 -> modifies loc_none h0 h1)
+let readLane s x y = s.(x +! size 5 *! y)
+
+inline_for_extraction noextract
+val writeLane:
+     s:state
+  -> x:index
+  -> y:index
+  -> v:uint64
+  -> Stack unit
+    (requires fun h -> live h s)
+    (ensures  fun h0 r h1 -> modifies (loc_buffer s) h0 h1)
+let writeLane s x y v = s.(x +! size 5 *! y) <- v
+
+val state_theta:
+     s:state
+  -> Stack unit
+    (requires fun h -> live h s)
+    (ensures  fun h0 _ h1 -> modifies (loc_buffer s) h0 h1)
+let state_theta s =
+  push_frame();
+  let _C:lbuffer uint64 5 = create (size 5) (u64 0) in
+  let h0 = ST.get () in
+  loop_nospec #h0 (size 5) _C
+  (fun x ->
+    _C.(x) <-
+      readLane s x (size 0) ^.
+      readLane s x (size 1) ^.
+      readLane s x (size 2) ^.
+      readLane s x (size 3) ^.
+      readLane s x (size 4)
+  );
+
+  let h0 = ST.get () in
+  loop_nospec #h0 (size 5) s
+  (fun x ->
+    let _D = _C.((x +. size 4) %. size 5) ^. (_C.((x +. size 1) %. size 5) <<<. u32 1) in
+    let h1 = ST.get () in
+    loop_nospec #h1 (size 5) s
+    (fun y ->
+      writeLane s x y (readLane s x y ^. _D)
+    )
+  );
+  pop_frame()
+
+val state_pi_rho:
+     s:state
+  -> Stack unit
+    (requires fun h -> live h s)
+    (ensures  fun h0 _ h1 -> modifies (loc_buffer s) h0 h1)
+let state_pi_rho s =
+  push_frame();
+  let x:lbuffer size_t 1 = create (size 1) (size 1) in
+  let y:lbuffer size_t 1 = create (size 1) (size 0) in
+  let current:lbuffer uint64 1 = create (size 1) (readLane s (size 1) (size 0)) in
+  let h0 = ST.get () in
+  Lib.Loops.for (size 0) (size 24)
+  (fun h1 t ->
+    live h1 x /\ live h1 y /\ live h1 current /\ live h1 s /\
+    //v (get h1 x 0) < 5 /\ v (get h1 y 0) < 5 /\
+    modifies (loc_union (loc_union (loc_buffer x) (loc_buffer y)) (loc_union (loc_buffer current) (loc_buffer s))) h0 h1)
+  (fun t ->
+    let h0 = ST.get () in
+    assume (v (get h0 x 0) < 5 /\ v (get h0 y 0) < 5);
+
+    let x0:index = x.(size 0) in
+    let y0:index = y.(size 0) in
+    let current0:uint64 = current.(size 0) in
+
+    let r : r:uint32{uint_v r < 64} = size_to_uint32 (((t +. size 1) *. (t +. size 2) /. size 2) %. size 64) in
+    let _Y:index = (size 2 *. x0 +. size 3 *. y0) %. size 5 in
+    let temp = readLane s y0 _Y in
+    assume (0 < uint_v r /\ uint_v r < 64);
+    writeLane s y0 _Y (current0 <<<. r);
+
+    x.(size 0) <- y0;
+    y.(size 0) <- _Y;
+    current.(size 0) <- temp
+  );
+  pop_frame()
+
+val state_chi:
+     s:state
+  -> Stack unit
+    (requires fun h -> live h s)
+    (ensures  fun h0 _ h1 -> modifies (loc_buffer s) h0 h1)
+let state_chi s =
+  push_frame ();
+  let temp:state = create (size 25) (u64 0) in
+  update_sub temp (size 0) (size 25) s;
+  let h0 = ST.get () in
+  loop_nospec #h0 (size 5) s
+  (fun y ->
+    let h1 = ST.get () in
+    loop_nospec #h1 (size 5) s
+    (fun x ->
+      writeLane s x y
+	(readLane temp x y ^.
+	((lognot (readLane temp ((x +. size 1) %. size 5) y)) &. readLane temp ((x +. size 2) %. size 5) y))
+    )
+  );
+  pop_frame ()
+
+val state_iota:
+     s:state
+  -> lfsr:uint8
+  -> Stack uint8
+    (requires fun h -> live h s)
+    (ensures  fun h0 _ h1 -> modifies (loc_buffer s) h0 h1)
+let state_iota s lfsr =
+  push_frame();
+  let lfsr:lbytes 1 = create (size 1) lfsr in
+  let h0 = ST.get () in
+  Lib.Loops.for (size 0) (size 7)
+  (fun h1 j ->
+    live h1 lfsr /\ live h1 s /\
+    modifies (loc_union (loc_buffer s) (loc_buffer lfsr)) h0 h1)
+  (fun j ->
+    let bitPosition = (u32 1 <<. size_to_uint32 j) -. u32 1 in
+    assume (uint_v bitPosition < 64);
+    let lfsr1, result = lfsr86540 lfsr.(size 0) in
+    (if result then
+      writeLane s (size 0) (size 0)
+	(readLane s (size 0) (size 0) ^. (u64 1 <<. bitPosition)));
+    lfsr.(size 0) <- lfsr1
+  );
+  let res = lfsr.(size 0) in
+  pop_frame();
+  res
+
+val state_permute1:
+     s:state
+  -> lfsr:uint8
+  -> Stack uint8
+    (requires fun h -> live h s)
+    (ensures  fun h0 _ h1 -> modifies (loc_buffer s) h0 h1)
+let state_permute1 s lfsr =
+  state_theta s;
+  state_pi_rho s;
+  state_chi s;
+  state_iota s lfsr
+
+val state_permute:
+     s:state
+  -> Stack unit
+    (requires fun h -> live h s)
+    (ensures  fun h0 _ h1 -> modifies (loc_buffer s) h0 h1)
+let state_permute s =
+  push_frame();
+  let lfsr:lbytes 1 = create (size 1) (u8 0x01) in
+  let h0 = ST.get () in
+  Lib.Loops.for (size 0) (size 24)
+  (fun h1 i ->
+    live h1 lfsr /\ live h1 s /\
+    modifies (loc_union (loc_buffer lfsr) (loc_buffer s)) h0 h1)
+  (fun i ->
+    lfsr.(size 0) <- state_permute1 s lfsr.(size 0)
+  );
+  pop_frame()
+
+#reset-options "--z3rlimit 50 --max_fuel 0 --max_ifuel 0"
+
+val loadState:
+     rateInBytes:size_t{v rateInBytes <= 200}
+  -> input:lbytes (v rateInBytes)
+  -> s:state
+  -> Stack unit
+    (requires fun h -> live h input /\ live h s /\ disjoint input s)
+    (ensures  fun h0 _ h1 -> modifies (loc_buffer s) h0 h1)
+let loadState rateInBytes input s =
+  push_frame();
+  let block:lbytes 200 = create (size 200) (u8 0) in
+  update_sub block (size 0) rateInBytes input;
+  let h0 = ST.get () in
+  Lib.Loops.for (size 0) (size 25)
+  (fun h1 j ->
+    live h1 block /\ live h1 s /\
+    modifies (loc_buffer s) h0 h1)
+  (fun j ->
+    s.(j) <- s.(j) ^. uint_from_bytes_le #U64 (sub #_ #200 #8 block (j *! size 8) (size 8))
+  );
+  pop_frame()
+
+val storeState:
+     rateInBytes:size_t{v rateInBytes <= 200}
+  -> s:state
+  -> res:lbytes (v rateInBytes)
+  -> Stack unit
+    (requires fun h -> live h s /\ live h res /\ disjoint s res)
+    (ensures  fun h0 _ h1 -> modifies (loc_buffer res) h0 h1)
+let storeState rateInBytes s res =
+  push_frame();
+  let block:lbytes 200 = create (size 200) (u8 0) in
+  let h0 = ST.get () in
+  loop_nospec #h0 (size 25) block
+  (fun j ->
+    uint_to_bytes_le (sub block (j *! size 8) (size 8)) s.(j)
+  );
+  update_sub res (size 0) rateInBytes (sub block (size 0) rateInBytes);
+  pop_frame()
+
+inline_for_extraction noextract
+val absorb_last:
+     s:state
+  -> rateInBytes:size_t{v rateInBytes > 0 /\ v rateInBytes <= 200}
+  -> inputByteLen:size_t
+  -> input:lbytes (v inputByteLen)
+  -> delimitedSuffix:uint8
+  -> Stack unit
+    (requires fun h -> live h s /\ live h input /\ disjoint s input)
+    (ensures  fun h0 _ h1 -> modifies (loc_buffer s) h0 h1)
+let absorb_last s rateInBytes inputByteLen input delimitedSuffix =
+  push_frame ();
+  let lastBlock = create rateInBytes (u8 0) in
+  let rem = inputByteLen %. rateInBytes in
+  let last = sub input (inputByteLen -. rem) rem in
+  update_sub lastBlock (size 0) rem last;
+  lastBlock.(rem) <- delimitedSuffix;
+  loadState rateInBytes lastBlock s;
+  pop_frame ()
+
+inline_for_extraction noextract
+val absorb_next:
+     s:state
+  -> rateInBytes:size_t{v rateInBytes > 0 /\ v rateInBytes <= 200}
+  -> Stack unit
+    (requires fun h -> live h s)
+    (ensures  fun h0 _ h1 -> modifies (loc_buffer s) h0 h1)
+let absorb_next s rateInBytes =
+  push_frame ();
+  let nextBlock = create rateInBytes (u8 0) in
+  nextBlock.(rateInBytes -! size 1) <- u8 0x80;
+  loadState rateInBytes nextBlock s;
+  state_permute s;
+  pop_frame ()
+
+val absorb:
+     s:state
+  -> rateInBytes:size_t{v rateInBytes > 0 /\ v rateInBytes <= 200}
+  -> inputByteLen:size_t
+  -> input:lbytes (v inputByteLen)
+  -> delimitedSuffix:uint8
+  -> Stack unit
+    (requires fun h -> live h s /\ live h input /\ disjoint s input)
+    (ensures  fun h0 _ h1 -> modifies (loc_buffer s) h0 h1)
+let absorb s rateInBytes inputByteLen input delimitedSuffix =
+  let open Lib.RawIntTypes in
+  let n = inputByteLen /. rateInBytes in
+  let rem = inputByteLen %. rateInBytes in
+  let h0 = ST.get () in
+  loop_nospec #h0 n s
+  (fun i ->
+    assume (v i * v rateInBytes + v rateInBytes <= v inputByteLen);
+    loadState rateInBytes (sub #_ #(v inputByteLen) #(v rateInBytes) input (i *! rateInBytes) rateInBytes) s;
+    state_permute s
+  );
+  absorb_last s rateInBytes inputByteLen input delimitedSuffix;
+  (if (not (u8_to_UInt8 (delimitedSuffix &. u8 0x80) = 0uy) && (size_to_UInt32 rem = size_to_UInt32 (rateInBytes -. size 1)))
+  then state_permute s);
+  absorb_next s rateInBytes
+
+val squeeze:
+     s:state
+  -> rateInBytes:size_t{v rateInBytes > 0 /\ v rateInBytes <= 200}
+  -> outputByteLen:size_t
+  -> output:lbytes (v outputByteLen)
+  -> Stack unit
+    (requires fun h -> live h s /\ live h output /\ disjoint s output)
+    (ensures  fun h0 _ h1 -> modifies (loc_union (loc_buffer s) (loc_buffer output)) h0 h1)
+let squeeze s rateInBytes outputByteLen output =
+  let outBlocks = outputByteLen /. rateInBytes in
+  let remOut = outputByteLen %. rateInBytes in
+  let h0 = ST.get () in
+  Lib.Loops.for (size 0) outBlocks
+  (fun h1 i ->
+    live h1 s /\ live h1 output /\
+    modifies (loc_union (loc_buffer s) (loc_buffer output)) h0 h1)
+  (fun i ->
+    assume (v i * v rateInBytes + v rateInBytes <= v outputByteLen);
+    storeState rateInBytes s (sub output (i *! rateInBytes) rateInBytes);
+    state_permute s
+  );
+  storeState remOut s (sub output (outputByteLen -. remOut) remOut)
+
+val keccak:
+     rate:size_t{v rate % 8 = 0 /\ v rate / 8 > 0 /\ v rate <= 1600}
+  -> capacity:size_t{v capacity + v rate == 1600}
+  -> inputByteLen:size_t
+  -> input:lbytes (v inputByteLen)
+  -> delimitedSuffix:uint8
+  -> outputByteLen:size_t
+  -> output:lbytes (v outputByteLen)
+  -> Stack unit
+    (requires fun h -> live h input /\ live h output /\ disjoint input output)
+    (ensures  fun h0 _ h1 -> modifies (loc_buffer output) h0 h1)
+let keccak rate capacity inputByteLen input delimitedSuffix outputByteLen output =
+  push_frame();
+  let rateInBytes = rate /. size 8 in
+  let s:state = create (size 25) (u64 0) in
+  absorb s rateInBytes inputByteLen input delimitedSuffix;
+  squeeze s rateInBytes outputByteLen output;
+  pop_frame()
