code/experimental/sha3/Hacl.SHA3.fst
@@ -1,0 +1,88 @@
+module Hacl.SHA3
+
+open FStar.HyperStack.All
+open FStar.HyperStack
+open FStar.HyperStack.ST
+open FStar.Mul
+
+open LowStar.Buffer
+
+open Lib.IntTypes
+open Lib.PQ.Buffer
+open Lib.Endianness
+
+open Hacl.Impl.SHA3
+
+module ST = FStar.HyperStack.ST
+module HS = FStar.HyperStack
+module B = LowStar.Buffer
+
+#reset-options "--z3rlimit 50 --max_fuel 0 --max_ifuel 0 --using_facts_from '* -FStar.Seq'"
+
+val shake128:
+     inputByteLen:size_t
+  -> input:lbytes (v inputByteLen)
+  -> outputByteLen:size_t
+  -> output:lbytes (v outputByteLen)
+  -> Stack unit
+     (requires fun h ->
+       live h input /\ live h output /\ disjoint input output)
+     (ensures  fun h0 _ h1 -> modifies (loc_buffer output) h0 h1)
+let shake128 inputByteLen input outputByteLen output =
+  keccak (size 1344) (size 256) inputByteLen input (u8 0x1F) outputByteLen output
+
+val shake256:
+     inputByteLen:size_t
+  -> input:lbytes (v inputByteLen)
+  -> outputByteLen:size_t
+  -> output:lbytes (v outputByteLen)
+  -> Stack unit
+     (requires fun h ->
+       live h input /\ live h output /\ disjoint input output)
+     (ensures  fun h0 _ h1 -> modifies (loc_buffer output) h0 h1)
+let shake256 inputByteLen input outputByteLen output =
+  keccak (size 1088) (size 512) inputByteLen input (u8 0x1F) outputByteLen output
+
+val sha3_224:
+     inputByteLen:size_t
+  -> input:lbytes (v inputByteLen)
+  -> output:lbytes 28
+  -> Stack unit
+     (requires fun h ->
+       live h input /\ live h output /\ disjoint input output)
+     (ensures  fun h0 _ h1 -> modifies (loc_buffer output) h0 h1)
+let sha3_224 inputByteLen input output =
+  keccak (size 1152) (size 448) inputByteLen input (u8 0x06) (size 28) output
+
+val sha3_256:
+     inputByteLen:size_t
+  -> input:lbytes (v inputByteLen)
+  -> output:lbytes 32
+  -> Stack unit
+     (requires fun h ->
+       live h input /\ live h output /\ disjoint input output)
+     (ensures  fun h0 _ h1 -> modifies (loc_buffer output) h0 h1)
+let sha3_256 inputByteLen input output =
+  keccak (size 1088) (size 512) inputByteLen input (u8 0x06) (size 32) output
+
+val sha3_384:
+     inputByteLen:size_t
+  -> input:lbytes (v inputByteLen)
+  -> output:lbytes 48
+  -> Stack unit
+     (requires fun h ->
+       live h input /\ live h output /\ disjoint input output)
+     (ensures  fun h0 _ h1 -> modifies (loc_buffer output) h0 h1)
+let sha3_384 inputByteLen input output =
+  keccak (size 832) (size 768) inputByteLen input (u8 0x06) (size 48) output
+
+val sha3_512:
+     inputByteLen:size_t
+  -> input:lbytes (v inputByteLen)
+  -> output:lbytes 64
+  -> Stack unit
+     (requires fun h ->
+       live h input /\ live h output /\ disjoint input output)
+     (ensures  fun h0 _ h1 -> modifies (loc_buffer output) h0 h1)
+let sha3_512 inputByteLen input output =
+  keccak (size 576) (size 1024) inputByteLen input (u8 0x06) (size 64) output
