specs/tests/Spec.Keccak.Test.fst
@@ -10,9 +10,9 @@ open Lib.ByteSequence
 
 let print_and_compare (len:size_nat) (test_expected:lbytes len) (test_result:lbytes len) =
   IO.print_string "\n\nResult:   ";
-  List.iter (fun a -> IO.print_string (UInt8.to_string_hex (u8_to_UInt8 a))) (as_list test_result);
+  List.iter (fun a -> IO.print_string (UInt8.to_string (u8_to_UInt8 a))) (as_list test_result);
   IO.print_string "\nExpected: ";
-  List.iter (fun a -> IO.print_string (UInt8.to_string_hex (u8_to_UInt8 a))) (as_list test_expected);
+  List.iter (fun a -> IO.print_string (UInt8.to_string (u8_to_UInt8 a))) (as_list test_expected);
   for_all2 (fun a b -> uint_to_nat #U8 a = uint_to_nat #U8 b) test_expected test_result
 
 
